src/lib/kuiper/types/Kuiper.Float32.fsti
@@ -3,6 +3,8 @@ module Kuiper.Float32
 open FStar.Tactics.Typeclasses { solve }
 open Kuiper.Sized
 open Kuiper.Scalars.Base
+open Kuiper.Floating.Base
+open Kuiper.Approximates.Base
 
 new
 val t : Type0
@@ -13,34 +15,35 @@ val one : t
 inline_for_extraction noextract
 instance _ : sized t = { size = 4sz; default = zero }
 
-val add : t -> t -> t
-val sub : t -> t -> t
-val mul : t -> t -> t
-val div : t -> t -> t
-
-val eq : t -> t -> bool
 val lt : t -> t -> bool
 val lte : t -> t -> bool
+val eq : t -> t -> bool
+
+val add : t -> t -> t
+val mul : t -> t -> t
+val sub : t -> t -> t
+val div : t -> t -> t
 
 val valid : t -> bool
 
-val lte_is_lt_or_eq (x y : t) :
-  Lemma (requires valid x /\ valid y) (ensures lte x y <==> lt x y \/ eq x y)
-
-val negate_lt_is_lte (x y : t) :
-  Lemma (requires valid x /\ valid y) (ensures lt x y <==> not (lte y x))
+val eq_spec (x y : t) (_ : (valid x /\ valid y)) : (eq x y <==> x == y)
+val lte_is_lt_or_eq (x y : t) (_ : (valid x /\ valid y)) : (lte x y <==> lt x y \/ eq x y)
+val negate_lt_is_lte (x y : t) (_ : (valid x /\ valid y)) : (lt x y <==> not (lte y x))
+val add_comm (x y : t) (_ : valid x) (_ : valid y) : (eq (add x y) (add y x))
+val mul_comm (x y : t) (_ : valid x) (_ : valid y) : (eq (mul x y) (mul y x))
+val add_zero (x : t) (_ : valid x) : (eq (add x zero) x)
 
 inline_for_extraction noextract
 instance _ : scalar t = {
   is_sized = solve;
   add; mul; zero; one; lt; lte; eq; valid;
-  lte_is_lt_or_eq; negate_lt_is_lte;
+  eq_spec; lte_is_lt_or_eq; negate_lt_is_lte;
+  add_comm; mul_comm; add_zero;
 }
 
 val exp : t -> t
 val log : t -> t
 
-(* Transcendental and math primitives *)
 val sqrt : t -> t
 val rsqrt : t -> t
 val sin : t -> t
@@ -61,7 +64,6 @@ val log2 : t -> t
 val log10 : t -> t
 val exp2 : t -> t
 
-(* Binary *)
 val pow : t -> t -> t
 val atan2 : t -> t -> t
 val fmin : t -> t -> t
@@ -69,7 +71,17 @@ val fmax : t -> t -> t
 val fmod : t -> t -> t
 val copysign : t -> t -> t
 
-(* Ternary *)
 val fma : t -> t -> t -> t
 
-val add_comm (x y : t) : Lemma (add x y == add y x) [SMTPat (add x y)]
+inline_for_extraction noextract
+instance _ : floating t = {
+  is_scalar = solve;
+  div; sub;
+  exp; log; sqrt; rsqrt; sin; cos; tan; asin; acos; atan;
+  sinh; cosh; tanh; ceil; floor; round; fabs; erf; log2;
+  log10; exp2; pow; atan2; fmin; fmax; fmod; copysign;
+  fma;
+}
+
+instance val is_real_like : real_like t
+instance val is_floating_real_like : floating_real_like t
