src/lib/kuiper/types/Kuiper.Floating.Base.fsti
@@ -1,0 +1,44 @@
+module Kuiper.Floating.Base
+
+open Kuiper.Scalars.Base
+open FStar.Tactics.Typeclasses { solve, tcinstance }
+
+inline_for_extraction noextract
+class floating (t : Type) = {
+  [@@@tcinstance]
+  is_scalar : scalar t;
+  sub : t -> t -> t;
+  div : t -> t -> t;
+  exp : t -> t;
+  log : t -> t;
+  sqrt : t -> t;
+  rsqrt : t -> t;
+  sin : t -> t;
+  cos : t -> t;
+  tan : t -> t;
+  asin : t -> t;
+  acos : t -> t;
+  atan : t -> t;
+  sinh : t -> t;
+  cosh : t -> t;
+  tanh : t -> t;
+  ceil : t -> t;
+  floor : t -> t;
+  round : t -> t;
+  fabs : t -> t;
+  erf : t -> t;
+  log2 : t -> t;
+  log10 : t -> t;
+  exp2 : t -> t;
+  pow : t -> t -> t;
+  atan2 : t -> t -> t;
+  fmin : t -> t -> t;
+  fmax : t -> t -> t;
+  fmod : t -> t -> t;
+  copysign : t -> t -> t;
+  fma : t -> t -> t -> t;
+}
+
+inline_for_extraction noextract
+let abs (#t:Type) {| floating t |} (x : t) : t =
+  if x `gte` zero then x else sub zero x
