src/lib/kuiper/types/Kuiper.Scalars.fst
@@ -1,3 +1,49 @@
 module Kuiper.Scalars
 
-(* Placeholder *)
+#set-options "--z3seed 1" // Sigh
+
+(* The default proofs here are very slow. *)
+
+inline_for_extraction noextract
+instance is_scalar_u8 : scalar UInt8.t =
+  let open FStar.UInt8 in
+  {
+    is_sized = solve;
+    add = add_mod;
+    mul = mul_mod;
+    zero; one; lt; lte; eq;
+    valid = (fun _ -> true);
+  }
+
+inline_for_extraction noextract
+instance is_scalar_u16 : scalar UInt16.t =
+  let open FStar.UInt16 in
+  {
+    is_sized = solve;
+    add = add_mod;
+    mul = mul_mod;
+    zero; one; lt; lte; eq;
+    valid = (fun _ -> true);
+  }
+
+inline_for_extraction noextract
+instance is_scalar_u32 : scalar UInt32.t =
+  let open FStar.UInt32 in
+  {
+    is_sized = solve;
+    add = add_mod;
+    mul = mul_mod;
+    zero; one; lt; lte; eq;
+    valid = (fun _ -> true);
+  }
+
+inline_for_extraction noextract
+instance is_scalar_u64 : scalar UInt64.t =
+  let open FStar.UInt64 in
+  {
+    is_sized = solve;
+    add = add_mod;
+    mul = mul_mod;
+    zero; one; lt; lte; eq;
+    valid = (fun _ -> true);
+  }
