src/lib/kuiper/types/Kuiper.Scalars.fsti
@@ -9,53 +9,13 @@ total unconditional operations on them. The instances for float types
 are in their own modules. *)
 
 inline_for_extraction noextract
-instance _ : scalar UInt8.t =
-  let open FStar.UInt8 in
-  {
-    is_sized = solve;
-    add = add_mod;
-    mul = mul_mod;
-    zero; one; lt; lte; eq;
-    valid = (fun _ -> true);
-    lte_is_lt_or_eq = (fun _ _ -> ());
-    negate_lt_is_lte = (fun _ _ -> ());
-  }
+instance val is_scalar_u8 : scalar UInt8.t
 
-inline_for_extraction
-instance _ : scalar UInt16.t =
-  let open FStar.UInt16 in
-  {
-    is_sized = solve;
-    add = add_mod;
-    mul = mul_mod;
-    zero; one; lt; lte; eq;
-    valid = (fun _ -> true);
-    lte_is_lt_or_eq = (fun _ _ -> ());
-    negate_lt_is_lte = (fun _ _ -> ());
-  }
+inline_for_extraction noextract
+instance val is_scalar_u16 : scalar UInt16.t
 
-inline_for_extraction
-instance _ : scalar UInt32.t =
-  let open FStar.UInt32 in
-  {
-    is_sized = solve;
-    add = add_mod;
-    mul = mul_mod;
-    zero; one; lt; lte; eq;
-    valid = (fun _ -> true);
-    lte_is_lt_or_eq = (fun _ _ -> ());
-    negate_lt_is_lte = (fun _ _ -> ());
-  }
+inline_for_extraction noextract
+instance val is_scalar_u32 : scalar UInt32.t
 
-inline_for_extraction
-instance _ : scalar UInt64.t =
-  let open FStar.UInt64 in
-  {
-    is_sized = solve;
-    add = add_mod;
-    mul = mul_mod;
-    zero; one; lt; lte; eq;
-    valid = (fun _ -> true);
-    lte_is_lt_or_eq = (fun _ _ -> ());
-    negate_lt_is_lte = (fun _ _ -> ());
-  }
+inline_for_extraction noextract
+instance val is_scalar_u64 : scalar UInt64.t
